added communications

ModularEngine/src/LogicEngine.FStar/net.fst
@@ -4,5 +4,33 @@ open Types
 type Received :: 'a::* => 'a => E
 assume forall (x:'a) (l:list 'a). In x l && Received l => Received x
 
+val methods: Ref (list (principal * (bool -> bytes) * (bytes -> bool)))
+let methods = newref []
+val suscribe: list (principal * (bool -> bytes) * (bytes -> bool)) -> unit
+let suscribe l = (methods:= l)
+
+val findMethod: principal -> list (principal * (bool -> bytes) * (bytes -> bool)) 
+    -> ((bool->bytes) * (bytes->bool))
+let rec findMethod p l = match l with
+  | [] -> raise (strcat "cannot find methods for " p)
+  | (p', recv, send_to) :: rest ->
+    if p = p' then (recv, send_to)
+    else findMethod p rest
+  
 val receive: unit -> b:bytes{Received b}
+let receive () =
+  let me = Crypto.lookup_my_credentials() in
+  match findMethod me (!methods) with
+    | (recv, _ ) ->
+      let b = recv true in
+      (assume (Received b); b)
+    | _ -> raise "Net.receive"
+  
 val send: principal -> bytes -> unit
+let send p b =
+  match findMethod p (!methods) with
+    | (_, send_to) ->
+      let _ = send_to b in
+      ()
+    | _ -> raise "Net.send"
+
