ModularEngine/src/LogicEngine.FStar/prims.fst
@@ -245,6 +245,9 @@ extern Runtime val strRmPfx: s:string -> pfx:string -> r:string{s=(Strcat pfx r)
 extern Runtime val strSplitByDelimiter: s:string -> d:string -> (r1:string*r2:string{(Strcat r1 r2)=s})
 extern Runtime val intCheckRange: int -> int -> int -> bool
 
+extern Runtime val createComm: int -> ((bool -> bytes) * (bytes -> bool))
+extern Runtime val stopAllServers: bool -> bool
+
 extern Runtime val boxToObject: 'a -> object
 extern Runtime val addBindings: object -> string -> bool
 (* extern Runtime val lookupBindings: object -> option string *)
